OpenvmFv/Spec/RTYPE/equivalence.lean
@@ -1,0 +1,333 @@
+import OpenvmFv.Spec.ALU
+import OpenvmFv.Spec.RTYPE.add
+
+namespace Equivalence.ALU
+
+  structure ALU_instruction_fields where
+    is_valid : FBB
+    non_imm : FBB
+
+    pc : FBB
+    next_pc : FBB
+
+    opcode : FBB
+
+    prev_a_timestamp : FBB
+    a_timestamp : FBB
+    prev_b_timestamp : FBB
+    b_timestamp : FBB
+    prev_c_timestamp : FBB
+    c_timestamp : FBB
+    timestamp : FBB
+    next_timestamp : FBB
+
+    rs1_ptr : FBB
+    rs2_ptr : FBB
+    rd_ptr : FBB
+
+    prev_a : Fin 4 → FBB
+    a : Fin 4 → FBB
+    b : Fin 4 → FBB
+    c : Fin 4 → FBB
+
+    range_checked_vals : Fin 6 → FBB
+    bitwise_vals : Fin 5 → Fin 4 → FBB
+
+  def wrap_to_word (vals : Fin 4 → FBB) : BitVec 32 :=
+    (@BabyBear.toU32
+      (vals 0 % 256)
+      (vals 1 % 256)
+      (vals 2 % 256)
+      (vals 3 % 256)
+      (by grind)).toBV
+
+  def is_normalized_word (vals : Fin 4 → FBB) : Prop :=
+    BabyBear.isU32
+      (vals 0)
+      (vals 1)
+      (vals 2)
+      (vals 3)
+
+  def wrap_to_regidx (val : FBB) : Fin 32 :=
+    ⟨val % 32, by grind⟩
+
+  def AddInput_of_ALU_instruction_fields (row : ALU_instruction_fields) : PureSpec.AddInput := {
+    r1_val := wrap_to_word row.b
+    r2_val := wrap_to_word row.c
+    rd := wrap_to_regidx row.rd_ptr
+    PC := row.pc.toNat
+    : PureSpec.AddInput
+  }
+
+  def AddOutput_matches_ALU_instruction_fields (row : ALU_instruction_fields) (add_output : PureSpec.AddOutput) : Prop :=
+    is_normalized_word row.b ∧
+    is_normalized_word row.c ∧
+    add_output.nextPC = row.next_pc.toNat ∧
+    match add_output.rd with
+      | .none => row.a = row.prev_a
+      | .some (rd, rd_val) =>
+        is_normalized_word row.a ∧
+        wrap_to_word row.a = rd_val ∧
+        rd.1.toNat = row.rd_ptr.toNat
+
+  def ALU_instruction_fields.spec (row : ALU_instruction_fields) : Prop :=
+    row.is_valid = 1 → (
+      row.opcode ∈ Finset.Icc 512 516 ∧
+      ((row.opcode = 512 ∧ row.non_imm = 1) → (
+        AddOutput_matches_ALU_instruction_fields
+          row
+          (PureSpec.execute_RTYPE_add_pure (AddInput_of_ALU_instruction_fields row))
+      ))
+    )
+
+  def ALU_instruction_fields.execution (row : ALU_instruction_fields) : List (FBB × List FBB) := [
+    (-row.is_valid, [row.pc, row.timestamp]),
+    (row.is_valid, [row.next_pc, row.next_timestamp])
+  ]
+
+  def ALU_instruction_fields.memory (row : ALU_instruction_fields) : List (FBB × List FBB) := [
+    (-row.is_valid, [1, row.rs1_ptr, row.b 0, row.b 1, row.b 2, row.b 3, row.prev_b_timestamp]),
+    ( row.is_valid, [1, row.rs1_ptr, row.b 0, row.b 1, row.b 2, row.b 3, row.b_timestamp]),
+    (-row.non_imm, [row.non_imm, row.rs2_ptr, row.c 0, row.c 1, row.c 2, row.c 3, row.prev_c_timestamp]),
+    ( row.non_imm, [row.non_imm, row.rs2_ptr, row.c 0, row.c 1, row.c 2, row.c 3, row.c_timestamp]),
+    (-row.is_valid, [1, row.rd_ptr, row.prev_a 0, row.prev_a 1, row.prev_a 2, row.prev_a 3, row.prev_a_timestamp]),
+    ( row.is_valid, [1, row.rd_ptr, row.a 0, row.a 1, row.a 2, row.a 3, row.a_timestamp]),
+  ]
+
+  def ALU_instruction_fields.range_checks (row : ALU_instruction_fields) : List (FBB × List FBB) := [
+    (row.is_valid, [row.range_checked_vals 0, 17]),
+    (row.is_valid, [row.range_checked_vals 1, 12]),
+    (row.non_imm, [row.range_checked_vals 2, 17]),
+    (row.non_imm, [row.range_checked_vals 3, 12]),
+    (row.is_valid, [row.range_checked_vals 4, 17]),
+    (row.is_valid, [row.range_checked_vals 5, 12]),
+  ]
+
+  def ALU_instruction_fields.read_instruction (row : ALU_instruction_fields) : List (FBB × List FBB) := [
+    (row.is_valid, [row.pc, row.opcode, row.rd_ptr, row.rs1_ptr, row.rs2_ptr, 1, row.non_imm, 0, 0])
+  ]
+
+  def ALU_instruction_fields.bitwise (row : ALU_instruction_fields) : List (FBB × List FBB) := [
+    (row.is_valid, [row.bitwise_vals 0 0, row.bitwise_vals 0 1, row.bitwise_vals 0 2, row.bitwise_vals 0 3]),
+    (row.is_valid, [row.bitwise_vals 1 0, row.bitwise_vals 1 1, row.bitwise_vals 1 2, row.bitwise_vals 1 3]),
+    (row.is_valid, [row.bitwise_vals 2 0, row.bitwise_vals 2 1, row.bitwise_vals 2 2, row.bitwise_vals 2 3]),
+    (row.is_valid, [row.bitwise_vals 3 0, row.bitwise_vals 3 1, row.bitwise_vals 3 2, row.bitwise_vals 3 3]),
+    (row.is_valid - row.non_imm, [row.bitwise_vals 4 0, row.bitwise_vals 4 1, row.bitwise_vals 4 2, row.bitwise_vals 4 3]),
+  ]
+
+  def bus_from_instruction_fields (rows : List ALU_instruction_fields) : ℕ → List (FBB × List FBB) :=
+    λ index =>
+      if index = ExecutionBus then            rows.flatMap ALU_instruction_fields.execution
+      else if index = MemoryBus then          rows.flatMap ALU_instruction_fields.memory
+      else if index = RangeCheckerBus then    rows.flatMap ALU_instruction_fields.range_checks
+      else if index = ReadInstructionBus then rows.flatMap ALU_instruction_fields.read_instruction
+      else if index = BitwiseBus then         rows.flatMap ALU_instruction_fields.bitwise
+      else []
+
+  def allHold_allRows [Field ExtF] (air : Valid_VmAirWrapper_alu FBB ExtF) : Prop :=
+    ∀ row : (Fin (air.last_row + 1)), VmAirWrapper_alu.constraints.allHold air row.1 (by grind)
+
+  def get_instruction_fields (air : Valid_VmAirWrapper_alu FBB ExtF) : List ALU_instruction_fields :=
+    (List.range (air.last_row + 1)).map (λ row => {
+      is_valid := air.core.is_valid row 0
+      non_imm := air.adapter.rs2_as row 0
+      pc := air.adapter.from_state.pc row 0
+      next_pc := air.adapter.from_state.pc row 0 + 4
+      opcode := (air.core.ctx row 0).instruction.opcode
+      prev_a_timestamp := air.adapter.writes_aux.base.prev_timestamp row 0
+      a_timestamp := air.adapter.from_state.timestamp row 0 + 2
+      prev_b_timestamp := air.adapter.reads_aux_0.base.prev_timestamp row 0
+      b_timestamp := air.adapter.from_state.timestamp row 0
+      prev_c_timestamp := air.adapter.reads_aux_1.base.prev_timestamp row 0
+      c_timestamp := air.adapter.from_state.timestamp row 0 + 1
+      timestamp := air.adapter.from_state.timestamp row 0
+      next_timestamp := air.adapter.from_state.timestamp row 0 + 3
+      rs1_ptr := air.adapter.rs1_ptr row 0
+      rs2_ptr := air.adapter.rs2 row 0
+      rd_ptr := air.adapter.rd_ptr row 0
+      prev_a := λ idx => match idx with
+        | 0 => air.adapter.writes_aux.prev_data_0 row 0
+        | 1 => air.adapter.writes_aux.prev_data_1 row 0
+        | 2 => air.adapter.writes_aux.prev_data_2 row 0
+        | 3 => air.adapter.writes_aux.prev_data_3 row 0
+      a := λ idx => match idx with
+        | 0 => air.core.a_0 row 0
+        | 1 => air.core.a_1 row 0
+        | 2 => air.core.a_2 row 0
+        | 3 => air.core.a_3 row 0
+      b := λ idx => match idx with
+        | 0 => air.core.b_0 row 0
+        | 1 => air.core.b_1 row 0
+        | 2 => air.core.b_2 row 0
+        | 3 => air.core.b_3 row 0
+      c := λ idx => match idx with
+        | 0 => air.core.c_0 row 0
+        | 1 => air.core.c_1 row 0
+        | 2 => air.core.c_2 row 0
+        | 3 => air.core.c_3 row 0
+      range_checked_vals := λ idx => match idx with
+        | 0 => air.adapter.reads_aux_0.base.timestamp_lt_aux.lower_decomp_0 row 0
+        | 1 => air.adapter.reads_aux_0.base.timestamp_lt_aux.lower_decomp_1 row 0
+        | 2 => air.adapter.reads_aux_1.base.timestamp_lt_aux.lower_decomp_0 row 0
+        | 3 => air.adapter.reads_aux_1.base.timestamp_lt_aux.lower_decomp_1 row 0
+        | 4 => air.adapter.writes_aux.base.timestamp_lt_aux.lower_decomp_0 row 0
+        | 5 => air.adapter.writes_aux.base.timestamp_lt_aux.lower_decomp_1 row 0
+      bitwise_vals := λ x y => match (x, y) with
+        | (0, 0) => air.core.x_0 row 0
+        | (0, 1) => air.core.y_0 row 0
+        | (0, 2) => air.core.x_xor_y_0 row 0
+        | (0, 3) => 1
+        | (1, 0) => air.core.x_1 row 0
+        | (1, 1) => air.core.y_1 row 0
+        | (1, 2) => air.core.x_xor_y_1 row 0
+        | (1, 3) => 1
+        | (2, 0) => air.core.x_2 row 0
+        | (2, 1) => air.core.y_2 row 0
+        | (2, 2) => air.core.x_xor_y_2 row 0
+        | (2, 3) => 1
+        | (3, 0) => air.core.x_3 row 0
+        | (3, 1) => air.core.y_3 row 0
+        | (3, 2) => air.core.x_xor_y_3 row 0
+        | (3, 3) => 1
+        | (4, 0) => air.core.c_0 row 0
+        | (4, 1) => air.core.c_1 row 0
+        | (4, 2) => 0
+        | (4, 3) => 0
+      : ALU_instruction_fields
+    })
+
+  theorem alu_spec [Field ExtF]
+    (air : Valid_VmAirWrapper_alu FBB ExtF)
+    (h_constraints : allHold_allRows air)
+    (h_bus_wellformedness : ∀ row ≤ air.last_row, VmAirWrapper_alu.constraints.wf_propertiesToAssumePerRow air row)
+  :
+    ∃ instruction_fields_list : List ALU_instruction_fields,
+      air.buses = bus_from_instruction_fields instruction_fields_list ∧
+      instruction_fields_list.Forall ALU_instruction_fields.spec
+  := by
+    have h_neg_one : (2013265920 : FBB) = (-1 : FBB) := rfl
+
+    have h_interactions := VmAirWrapper_alu.constraints.constrain_interactions_of_extraction air (h_constraints 0).1
+    unfold allHold_allRows at h_constraints
+    use get_instruction_fields air
+    split_ands
+    . unfold VmAirWrapper_alu.constraints.constrain_interactions at h_interactions
+      rewrite [h_interactions]; clear h_interactions
+      unfold bus_from_instruction_fields ALU_instruction_fields.execution ALU_instruction_fields.memory ALU_instruction_fields.range_checks ALU_instruction_fields.read_instruction ALU_instruction_fields.bitwise
+      simp [
+        get_instruction_fields,
+        VmAirWrapper_alu_constraint_and_interaction_simplification
+      ]
+      unfold VmAirWrapper_alu.constraints.executionBus_row
+      unfold VmAirWrapper_alu.constraints.memoryBus_row
+      unfold VmAirWrapper_alu.constraints.rangeCheckerBus_row
+      unfold VmAirWrapper_alu.constraints.readInstructionBus_row
+      unfold VmAirWrapper_alu.constraints.bitwiseBus_row
+      funext index
+      by_cases h_index: index = ExecutionBus
+      . simp [h_index, List.flatMap_map]
+      by_cases h_index: index = MemoryBus
+      . simp [h_index, List.flatMap_map]
+        congr
+        funext row
+        congr
+        all_goals simp [h_neg_one]
+      by_cases h_index: index = RangeCheckerBus
+      . simp [h_index, List.flatMap_map]
+      by_cases h_index: index = ReadInstructionBus
+      . simp [h_index, List.flatMap_map]
+      by_cases h_index: index = BitwiseBus
+      . simp [h_index, List.flatMap_map]
+      . simp [*]
+      done
+    . apply List.forall_iff_forall_mem.mpr
+      intro instruction_fields h_instruction_fields
+      unfold ALU_instruction_fields.spec
+      simp [get_instruction_fields] at h_instruction_fields
+      obtain ⟨row, ⟨h_row_range, h_fields⟩⟩ := h_instruction_fields
+      rewrite [←h_fields]; clear h_fields
+      simp
+
+      intro h_is_valid
+
+      have non_imm_spec := ALU.ValidRows.spec_base_ALU_non_imm
+        ExtF
+        air
+        row
+        (by omega)
+        (h_constraints ⟨row, by omega⟩)
+        h_is_valid
+        (h_bus_wellformedness row (by omega))
+
+      have ⟨
+        ⟨h_a0, h_a1, h_a2, h_a3, h_b0, h_b1, h_b2, h_b3, h_c0, h_c1, h_c2, h_c3⟩,
+        h_opcodes,
+        h_imm_binary,
+        h_imm_op_properties
+      ⟩ := ALU.ValidRows.essentials
+        ExtF
+        air
+        row
+        (by omega)
+        (h_constraints ⟨row, by omega⟩)
+        h_is_valid
+        (h_bus_wellformedness row (by omega))
+
+      dsimp only at *
+
+      split_ands
+      . grind
+      . grind
+      . intro h_opcode h_non_imm
+        simp [AddOutput_matches_ALU_instruction_fields]
+        split_ands
+        . assumption
+        . assumption
+        . assumption
+        . assumption
+        . assumption
+        . assumption
+        . assumption
+        . assumption
+        . simp [AddInput_of_ALU_instruction_fields, wrap_to_word, PureSpec.execute_RTYPE_add_pure]
+          sorry
+        . simp [AddInput_of_ALU_instruction_fields, wrap_to_word, PureSpec.execute_RTYPE_add_pure]
+          rewrite [dite_cond_eq_false]
+          . simp
+            split_ands
+            . assumption
+            . assumption
+            . assumption
+            . assumption
+            . specialize non_imm_spec h_non_imm
+              unfold execute_RTYPE_pure at non_imm_spec
+              simp only [h_opcode, ALU.ValidRows.rop_of_ALU_opcode] at non_imm_spec
+              dsimp at non_imm_spec
+              simp [
+                Nat.mod_eq_of_lt h_a0,
+                Nat.mod_eq_of_lt h_a1,
+                Nat.mod_eq_of_lt h_a2,
+                Nat.mod_eq_of_lt h_a3,
+                Nat.mod_eq_of_lt h_b0,
+                Nat.mod_eq_of_lt h_b1,
+                Nat.mod_eq_of_lt h_b2,
+                Nat.mod_eq_of_lt h_b3,
+                Nat.mod_eq_of_lt h_c0,
+                Nat.mod_eq_of_lt h_c1,
+                Nat.mod_eq_of_lt h_c2,
+                Nat.mod_eq_of_lt h_c3,
+              ]
+              rewrite [add_comm]
+              convert non_imm_spec using 7
+              . simp [Nat.mod_eq_of_lt h_a0]
+              . simp [Fin.ext_iff, Nat.mod_eq_of_lt h_a1]
+              simp [execute_RTYPE_pure, h_opcode, ALU.ValidRows.rop_of_ALU_opcode]
+              done
+            done
+          . -- rd != 0
+            done
+          done
+      done
+    done
+
+end Equivalence.ALU
