OpenvmFv/Spec/RTYPE/local.lean
@@ -31,21 +31,4 @@ namespace Local
     execute_RTYPE = LeanRV32D.Functions.execute_RTYPE
   := rfl
 
-  def execute_ITYPE (imm : (BitVec 12)) (rs1 : regidx) (rd : regidx) (op : iop) : SailM ExecutionResult := do
-    let immext : xlenbits := (LeanRV32D.Functions.sign_extend (m := 32) imm)
-    (LeanRV32D.Functions.wX_bits rd
-      (← do
-        match op with
-        | .ADDI => (pure ((← (LeanRV32D.Functions.rX_bits rs1)) + immext))
-        | .SLTI => (pure (LeanRV32D.Functions.zero_extend (m := 32) (LeanRV32D.Functions.bool_to_bits (LeanRV32D.Functions.zopz0zI_s (← (LeanRV32D.Functions.rX_bits rs1)) immext))))
-        | .SLTIU =>
-          (pure (LeanRV32D.Functions.zero_extend (m := 32) (LeanRV32D.Functions.bool_to_bits (LeanRV32D.Functions.zopz0zI_u (← (LeanRV32D.Functions.rX_bits rs1)) immext))))
-        | .ANDI => (pure ((← (LeanRV32D.Functions.rX_bits rs1)) &&& immext))
-        | .ORI => (pure ((← (LeanRV32D.Functions.rX_bits rs1)) ||| immext))
-        | .XORI => (pure ((← (LeanRV32D.Functions.rX_bits rs1)) ^^^ immext))))
-    (pure LeanRV32D.Functions.RETIRE_SUCCESS)
-
-  lemma execute_ITYPE_equiv :
-    execute_ITYPE = LeanRV32D.Functions.execute_ITYPE
-  := rfl
 end Local
